theories/examples/awkward_example_helpers.v
@@ -3,13 +3,99 @@ From iris.base_logic Require Import invariants.
 Require Import Eqdep_dec.
 From cap_machine Require Import
      rules logrel region_invariants fundamental region_invariants_revocation region_invariants_static.
+From cap_machine.examples Require Export stdpp_extra iris_extra.
 
+
+(* Helper definitions for creating static regions *)
+Definition lists_to_static_region (l1: list Addr) (l2: list Word): gmap Addr Word :=
+  list_to_map (zip l1 l2).
+
+Lemma lists_to_static_region_cons a w l1 l2 :
+  lists_to_static_region (a :: l1) (w :: l2) =
+  <[ a := w ]> (lists_to_static_region l1 l2).
+Proof. reflexivity. Qed.
+
+
+Lemma lists_to_static_region_lookup_None l1 l2 a :
+  a ∉ l1 → lists_to_static_region l1 l2 !! a = None.
+Proof.
+  revert l2. induction l1; eauto; []. intros l2 [? ?]%not_elem_of_cons.
+  destruct l2.
+  { cbn. eauto. }
+  { rewrite lists_to_static_region_cons. rewrite lookup_insert_None. eauto. }
+Qed.
+    
+Lemma lists_to_static_region_dom l1 l2 :
+  length l1 = length l2 →
+  dom (gset Addr) (lists_to_static_region l1 l2) = list_to_set l1.
+Proof.
+  intros Hlen. apply elem_of_equiv_L. intros x.
+  rewrite /lists_to_static_region elem_of_dom elem_of_list_to_set.
+  split. by intros [? ?%elem_of_list_to_map_2%elem_of_zip_l].
+  intros Hx.
+  destruct (elem_of_list_lookup_1 _ _ Hx) as [xi Hxi].
+  pose proof (lookup_lt_Some _ _ _ Hxi).
+  rewrite list_to_map_lookup_is_Some fst_zip //. lia.
+Qed.
+
+Lemma lists_to_static_region_size l1 l2 :
+  length l1 = length l2 → NoDup l1 ->
+  size (lists_to_static_region l1 l2) = length l1.
+Proof.
+  revert l2. 
+  induction l1;intros l2 Hlen Hdup.
+  - simpl. auto.
+  - simpl. destruct l2;inversion Hlen. apply NoDup_cons in Hdup as [Hnin Hdup]. 
+    rewrite -(IHl1 l2);auto.
+    rewrite /lists_to_static_region /=. rewrite map_size_insert;auto. 
+    apply not_elem_of_list_to_map_1. rewrite fst_zip;[auto|lia].
+Qed. 
+
+Lemma big_sepL2_to_static_region {Σ: gFunctors} l1 l2 (Φ : _ → _ → iProp Σ) Ψ :
+  NoDup l1 →
+  □ (∀ k a w, ⌜l1 !! k = Some a⌝ -∗ ⌜l2 !! k = Some w⌝ -∗ Φ a w -∗ Ψ a w) -∗
+  ([∗ list] a;w ∈ l1;l2, Φ a w) -∗
+  ([∗ map] a↦pv ∈ lists_to_static_region l1 l2, Ψ a pv).
+Proof.
+  revert l2. induction l1; intros l2 ND.
+  { cbn in *. iIntros "_ _". by iApply big_sepM_empty. }
+  { iIntros "#Ha H". iDestruct (big_sepL2_cons_inv_l with "H") as (w l2' ->) "[HΦ H]".
+    rewrite lists_to_static_region_cons. iApply big_sepM_insert.
+      by apply lists_to_static_region_lookup_None, NoDup_cons_11.
+    iSplitL "HΦ". { iApply ("Ha" $! 0); try (iPureIntro; apply cons_lookup); eauto. }
+    iApply IHl1; auto.
+    by eauto using NoDup_cons_12.
+    iModIntro. iIntros. iApply ("Ha" $! (S k)); auto. }
+Qed.
+
+Lemma static_region_to_big_sepL2 {Σ: gFunctors} l1 l2 (Φ : _ → _ -> iProp Σ) Ψ :
+  NoDup l1 → length l1 = length l2 ->
+  □ (∀ k a w, ⌜l1 !! k = Some a⌝ -∗ ⌜l2 !! k = Some w⌝ -∗ Ψ a w -∗ Φ a w) -∗
+  ([∗ map] a↦pv ∈ lists_to_static_region l1 l2, Ψ a pv) -∗
+  ([∗ list] a;w ∈ l1;l2, Φ a w).
+Proof.
+  revert l2. induction l1; intros l2 ND Hlen.
+  { cbn in *. iIntros "_ _". destruct l2;[|inversion Hlen]. done. }
+  { iIntros "#Ha H". destruct l2;[inversion Hlen|]. iDestruct (big_sepM_delete with "H") as "[Hψ H]".
+    rewrite lists_to_static_region_cons. apply lookup_insert.
+    iSplitL "Hψ". { iApply ("Ha" $! 0); try (iPureIntro; constructor). auto. }
+    iApply IHl1; auto.
+    by eauto using NoDup_cons_12.
+    iModIntro. iIntros. iApply ("Ha" $! (S k)); auto; iPureIntro.
+    rewrite lists_to_static_region_cons.
+    rewrite delete_insert. auto. by apply lists_to_static_region_lookup_None, NoDup_cons_11. }
+Qed.
 
 Section awkward_helpers.
   Context {Σ:gFunctors} {memg:memG Σ} {regg:regG Σ}
           {stsg : STSG Addr region_type Σ} {heapg : heapG Σ}
           `{MonRef: MonRefG (leibnizO _) CapR_rtc Σ} {nainv: logrel_na_invs Σ}
           `{MP: MachineParameters}.
+
+  Notation STS := (leibnizO (STS_states * STS_rels)).
+  Notation STS_STD := (leibnizO (STS_std_states Addr region_type)).
+  Notation WORLD := (prodO STS_STD STS). 
+  Implicit Types W : WORLD.
 
   Ltac iPrologue prog :=
     iDestruct prog as "[Hi Hprog]";
@@ -18,27 +104,6 @@ Section awkward_helpers.
   Ltac iEpilogue prog :=
     iNext; iIntros prog; iSimpl;
     iApply wp_pure_step_later;auto;iNext.
-
-  (* TODO: put into revocation file *)
-  Lemma related_sts_pub_world_fresh_loc W (i x : positive) r1 r2 :
-    i ∉ dom (gset positive) (loc W).1 →
-    i ∉ dom (gset positive) (loc W).2 →
-    related_sts_pub_world W (W.1,(<[i:=x]> W.2.1, <[i:= (r1,r2)]> W.2.2)).
-  Proof.
-    rewrite /loc. intros Hdom_sta Hdom_rel.
-    rewrite /related_sts_pub_world /=.
-    split;[apply related_sts_std_pub_refl|].
-    rewrite /related_sts_pub. split;[|split].
-    - rewrite dom_insert_L. set_solver.
-    - rewrite dom_insert_L. set_solver.
-    - apply (not_elem_of_dom (D:=gset positive) W.2.1 i) in Hdom_sta.
-      apply (not_elem_of_dom (D:=gset positive) W.2.2 i) in Hdom_rel.
-      intros j r1' r2' r1'' r2'' Hr' Hr''.
-      destruct (decide (j = i)).
-      + subst. rewrite Hdom_rel in Hr'. inversion Hr'.
-      + simplify_map_eq. repeat split;auto.
-        intros x' y Hx' Hy. simplify_map_eq. left. 
-  Qed.
 
   Lemma updatePcPerm_RX w g b e a :
     inr (RX, g, b, e, a) = updatePcPerm w ->
@@ -101,7 +166,222 @@ Section awkward_helpers.
       iApply (wp_bind (fill [SeqCtx])).
       iApply (wp_notCorrectPC with "HPC");eauto. 
       iEpilogue "_". iApply wp_value. iFrame.
-  Qed. 
+  Qed.
+
+
+  (* Lemma which splits a list of temp resources into its persistent and non persistent parts *)
+   Lemma temp_resources_split l W : 
+     ([∗ list] a ∈ l, (∃ (p : Perm) (φ : WORLD * Word → iPropI Σ),
+                          ⌜∀ Wv : WORLD * Word, Persistent (φ Wv)⌝ ∗ temp_resources W φ a p ∗ rel a p φ)
+                        ∗ ⌜std (revoke W) !! a = Some Revoked⌝) -∗
+     ∃ (ws : list Word), □ ([∗ list] a;w ∈ l;ws, ∃ p φ, ⌜∀ Wv : WORLD * Word, Persistent (φ Wv)⌝
+                                                             ∗ ⌜p ≠ O⌝
+                                                             ∗ φ (W,w)
+                                                             ∗ rel a p φ
+                                                             ∗ (if pwl p then future_pub_mono φ w
+                                                                else future_priv_mono φ w))
+                          ∗ ⌜Forall (λ a, std (revoke W) !! a = Some Revoked) l⌝
+                          ∗ ([∗ list] a;w ∈ l;ws, ∃ p φ, a ↦ₐ[p] w ∗ rel a p φ).
+   Proof.
+     rewrite /temp_resources. 
+     iIntros "Hl".
+     iAssert ([∗ list] a ∈ l, ∃ (v : Word), (∃ (p : Perm) (φ : WORLD * Word → iPropI Σ), 
+                            ⌜∀ Wv : WORLD * Word, Persistent (φ Wv)⌝
+                            ∗ ⌜p ≠ O⌝
+                            ∗ a ↦ₐ[p] v ∗ (if pwl p then future_pub_mono φ v else future_priv_mono φ v) ∗ φ (W, v)
+                            ∗ rel a p φ ∗ ⌜std (revoke W) !! a = Some Revoked⌝))%I
+       with "[Hl]" as "Hl".
+     { iApply (big_sepL_mono with "Hl").
+       iIntros (k y Hy) "Hy".
+       iDestruct "Hy" as "[Hy Hy']".
+       iDestruct "Hy" as (p φ) "(Hpers & Hv & Hrel)".
+       iDestruct "Hv" as (v) "(Hne & Hy & Hmono & Hφ)".
+       iExists v,p,φ. iFrame. 
+     }
+     iDestruct (region_addrs_exists with "Hl") as (wps) "Hl".
+     iExists wps. iSplit. 
+     - iAssert ([∗ list] a;w ∈ l;wps, ∃ p φ, ⌜∀ Wv : WORLD * Word, Persistent (φ Wv)⌝
+                                                             ∗ ⌜p ≠ O⌝
+                                                             ∗ φ (W,w)
+                                                             ∗ rel a p φ
+                                                             ∗ (if pwl p then future_pub_mono φ w
+                                                                else future_priv_mono φ w))%I
+         with "[Hl]" as "Hl". 
+       { iApply (big_sepL2_mono with "Hl").
+         iIntros (k y1 y2 Hy1 Hy2) "Hy".
+         iDestruct "Hy" as (p φ) "(Hpers & Hne & Hy & Hmono & Hφ & Hrel & Hrev)".
+         iExists p,φ. iFrame. 
+       }
+       iDestruct (region_addrs_exists2 with "Hl") as (ps Hlen) "Hl".
+       iDestruct (region_addrs_exists2 with "Hl") as (φs Hlen') "Hl".
+       iDestruct (big_sepL2_sep with "Hl") as "[Hpers Hl]".
+       iDestruct (big_sepL2_length with "Hl") as %Hlength. 
+       iDestruct (big_sepL2_to_big_sepL_r with "Hpers") as "Hpers";auto. 
+       iDestruct (big_sepL_forall with "Hpers") as %Hpers.
+       iAssert ([∗ list] y1;y2 ∈ l;zip (zip wps ps) φs, □ (⌜y2.1.2 ≠ O⌝
+                                                 ∗ y2.2 (W, y2.1.1)
+                                                   ∗ rel y1 y2.1.2 y2.2
+                                                     ∗ (if pwl y2.1.2
+                                                        then future_pub_mono y2.2 y2.1.1
+                                                        else future_priv_mono y2.2 y2.1.1)))%I
+         with "[Hl]" as "Hl".
+       { iApply (big_sepL2_mono with "Hl").
+         iIntros (k y1 y2 Hy1 Hy2) "Hy".
+         apply Hpers with (Wv:=(W,y2.1.1)) in Hy2.
+         destruct (pwl y2.1.2) eqn:Hpwl.
+         - iDestruct "Hy" as "#(Hne & Hy & Hrel & Hmono)".
+           iAlways. iFrame "#".
+         - iDestruct "Hy" as "#(Hne & Hy & Hrel & Hmono)".
+           iAlways. iFrame "#".
+       }
+       iDestruct "Hl" as "#Hl". 
+       iAlways. iApply region_addrs_exists2.
+       iExists ps. iSplit;auto. iApply region_addrs_exists2.
+       iExists φs. iSplit;auto.
+       iApply big_sepL2_sep. iSplit.
+       + iApply big_sepL2_to_big_sepL_r;auto. iApply big_sepL_forall. auto.
+       + iApply (big_sepL2_mono with "Hl").
+         iIntros (k y1 y2 Hy1 Hy2) "Hy".
+         iDestruct "Hy" as "#(Hne & Hy & Hrel & Hmono)".
+         iFrame "#".
+     - iAssert ([∗ list] a0;c0 ∈ l;wps, (∃ p (φ : WORLD * Word → iPropI Σ),
+                                    ⌜∀ Wv : WORLD * Word, Persistent (φ Wv)⌝
+                                    ∗ ⌜p ≠ O⌝
+                                      ∗ a0 ↦ₐ[p] c0
+                                        ∗ (if pwl p then future_pub_mono φ c0 else future_priv_mono φ c0)
+                                          ∗ φ (W, c0)
+                                            ∗ rel a0 p φ)
+                                              ∗ ⌜std (revoke W) !! a0 = Some Revoked⌝)%I
+         with "[Hl]" as "Hl".
+       { iApply (big_sepL2_mono with "Hl").
+         iIntros (k y1 y2 Hy1 Hy2) "Hy".
+         iDestruct "Hy" as (p φ) "(?&?&?&?&?&?&?)".
+         iFrame. iExists _,_. iFrame. 
+       }
+       iDestruct (big_sepL2_sep with "Hl") as "[Hl #Hrev]".
+       iDestruct (big_sepL2_length with "Hl") as %Hlength.
+       iSplit.
+       + iDestruct (big_sepL2_to_big_sepL_l with "Hrev") as "Hrev'";auto. 
+         iDestruct (big_sepL_forall with "Hrev'") as %Hrev.
+         iPureIntro. apply Forall_forall. intros x Hin.
+         apply elem_of_list_lookup in Hin as [k Hin].
+           by apply Hrev with (x:=k).
+       + iApply (big_sepL2_mono with "Hl").
+         iIntros (k y1 y2 Hy1 Hy2) "Hy".
+         iDestruct "Hy" as (p φ) "(?&?&?&?&?&?)". iExists _,_. 
+         iFrame.
+   Qed.
+
+   
+   (* ---------------------------------------------------------------------------------------------- *)
+   (* ------------------------------------ Awkward Invariant --------------------------------------- *)
+   (* ---------------------------------------------------------------------------------------------- *)
+
+   Definition awk_inv i a :=
+     (∃ x:bool, sts_state_loc (A:=Addr) i x
+           ∗ if x
+             then a ↦ₐ[RWX] inl 1%Z
+             else a ↦ₐ[RWX] inl 0%Z)%I.
+
+   Definition awk_rel_pub := λ a b, a = false ∨ b = true.
+   Definition awk_rel_priv := λ (a b : bool), True.
+
+   (* useful lemma about awk rels *)
+   Lemma rtc_rel_pub y x :
+     y = (encode true) ->
+     rtc (convert_rel awk_rel_pub) y x ->
+     x = (encode true).
+   Proof.
+     intros Heq Hrtc.
+     induction Hrtc; auto. 
+     rewrite Heq in H. 
+     inversion H as [y' [b [Heq1 [Heq2 Hy] ] ] ].
+     inversion Hy; subst; auto.
+     apply encode_inj in Heq1. inversion Heq1.
+   Qed.
+   Lemma rtc_rel_pub' x :
+     rtc (convert_rel awk_rel_pub) (encode true) (encode x) ->
+     x = true.
+   Proof.
+     intros Hrtc. 
+     apply encode_inj.
+     apply rtc_rel_pub with (encode true); auto.
+   Qed.
+   Lemma rtc_rel_pub_false y x :
+     y = (encode false) ->
+     rtc (convert_rel awk_rel_pub) y x ->
+     x = (encode true) ∨ x = (encode false).
+   Proof.
+     intros Heq Hrtc.
+     induction Hrtc; auto. 
+     rewrite Heq in H. 
+     inversion H as [y' [b [Heq1 [Heq2 Hy] ] ] ]. subst. 
+     destruct b;apply encode_inj in Heq1;auto;subst. 
+     left. eapply rtc_rel_pub; eauto. 
+   Qed.
+     
+   Definition awk_W W i : WORLD := (W.1,(<[i:=encode false]>W.2.1,<[i:=(convert_rel awk_rel_pub,convert_rel awk_rel_priv)]>W.2.2)).
+
+   (* namespace definitions for the regions *)
+   Definition regN : namespace := nroot .@ "regN".
+
+   (* The proof of the awkward example goes through a number of worlds.
+      Below are some helper lemmas and definitions about how these worlds 
+      are related *)
+   Lemma related_priv_local_1 W i :
+     W.2.1 !! i = Some (encode true) ->
+     W.2.2 !! i = Some (convert_rel awk_rel_pub, convert_rel awk_rel_priv) ->
+     related_sts_priv_world W (W.1, (<[i:=encode false]> W.2.1, W.2.2)).
+   Proof.
+     intros Hlookup Hrel. 
+     split;[apply related_sts_std_priv_refl|simpl].
+     split;[apply dom_insert_subseteq|split;[auto|] ].
+     intros j r1 r2 r1' r2' Hr Hr'.
+     rewrite Hr in Hr'. inversion Hr'; subst; repeat (split;auto).
+     intros x y Hx Hy.
+     destruct (decide (i = j)).
+     - subst. rewrite lookup_insert in Hy; inversion Hy; subst.
+       rewrite Hrel in Hr. rewrite Hlookup in Hx. inversion Hr; inversion Hx; subst.
+       right with (encode false);[|left].
+       right. exists true,false. repeat (split;auto).
+     - rewrite lookup_insert_ne in Hy;auto. rewrite Hx in Hy; inversion Hy; subst. left.
+   Qed.
+
+   Lemma related_pub_local_1 Wloc i (x : bool) :
+     Wloc.1 !! i = Some (encode x) ->
+     Wloc.2 !! i = Some (convert_rel awk_rel_pub, convert_rel awk_rel_priv) ->
+     related_sts_pub Wloc.1 (<[i:=encode true]> Wloc.1) Wloc.2 Wloc.2.
+   Proof.
+     intros Hx Hrel.
+     split;[apply dom_insert_subseteq|split;[auto|] ].
+     intros j r1 r2 r1' r2' Hr Hr'.
+     rewrite Hr in Hr'. inversion Hr'; subst; repeat (split;auto).
+     intros x' y Hx' Hy.
+     destruct (decide (i = j)).
+     - subst. rewrite lookup_insert in Hy; inversion Hy; subst.
+       rewrite Hrel in Hr. rewrite Hx in Hx'. inversion Hr; inversion Hx; subst.
+       right with (encode true);[|left].
+       exists x,true. inversion Hx'. subst. repeat (split;auto).
+       destruct x; rewrite /awk_rel_pub; auto. 
+     - rewrite lookup_insert_ne in Hy;auto. rewrite Hx' in Hy; inversion Hy; subst. left.
+   Qed.
+
+   Lemma related_pub_lookup_local W W' i x :
+     related_sts_pub_world W W' ->
+     W.2.1 !! i = Some (encode true) ->
+     W.2.2 !! i = Some (convert_rel awk_rel_pub, convert_rel awk_rel_priv) ->
+     W'.2.1 !! i = Some (encode x) -> x = true.
+   Proof.
+     intros Hrelated Hi Hr Hi'.
+     destruct Hrelated as [_ [Hdom1 [Hdom2 Htrans] ] ].
+     assert (is_Some (W'.2.2 !! i)) as [r' Hr'].
+     { apply elem_of_gmap_dom. apply elem_of_subseteq in Hdom2. apply Hdom2.
+       apply elem_of_gmap_dom. eauto. }
+     destruct r' as [r1' r2']. 
+     specialize (Htrans i _ _ _ _ Hr Hr') as [Heq1 [Heq2 Htrans] ].
+     subst. specialize (Htrans _ _ Hi Hi').
+     apply rtc_rel_pub'; auto. 
+   Qed.
 
 
 End awkward_helpers. 
