theories/examples/stdpp_extra.v
@@ -1,0 +1,56 @@
+From stdpp Require Import countable.
+From iris.base_logic Require Import invariants.
+
+Lemma elements_list_to_set {A} `{Countable A} (l: list A) :
+  NoDup l →
+  elements (list_to_set l : gset A) ≡ₚ l.
+Proof.
+  induction l.
+  - intros. rewrite list_to_set_nil elements_empty //.
+  - intros ND. rewrite list_to_set_cons elements_union_singleton.
+    + rewrite IHl //. eauto using NoDup_cons_12.
+    + rewrite not_elem_of_list_to_set. by apply NoDup_cons_11.
+Qed.
+
+Lemma list_to_map_lookup_is_Some {A B} `{Countable A, EqDecision A} (l: list (A * B)) (a: A) :
+  is_Some ((list_to_map l : gmap A B) !! a) ↔ a ∈ l.*1.
+Proof.
+  induction l.
+  - cbn. split; by inversion 1.
+  - cbn. rewrite lookup_insert_is_Some' elem_of_cons.
+    split; intros [HH|HH]; eauto; rewrite -> IHl in *; auto.
+Qed.
+
+Lemma zip_app {A B} (l1 l1': list A) (l2 l2' : list B) :
+  length l1 = length l2 ->
+  zip (l1 ++ l1') (l2 ++ l2') = zip l1 l2 ++ zip l1' l2'.
+Proof.
+  revert l2. induction l1;intros l2 Hlen.
+  - destruct l2;[|inversion Hlen]. done.
+  - destruct l2;[inversion Hlen|]. simpl.
+    f_equiv. auto. 
+Qed.
+
+Lemma length_zip_l {A B} (l1: list A) (l2: list B) :
+  length l1 ≤ length l2 → length (zip l1 l2) = length l1.
+Proof.
+  revert l2. induction l1; intros l2 Hl2; auto.
+  destruct l2; cbn in Hl2. exfalso; lia.
+  cbn. rewrite IHl1; auto. lia.
+Qed.
+
+Lemma list_filter_app { A: Type } (P: A -> Prop) `{ forall x, Decision (P x) } l1 l2:
+  @list_filter _ P _ (l1 ++ l2) = @list_filter _ P _ l1 ++ @list_filter _ P _ l2.
+Proof.
+  induction l1; simpl; auto.
+  destruct (decide (P a)); auto.
+  unfold filter. rewrite IHl1. auto.
+Qed.
+
+Lemma list_filter_forall { A: Type } (P: A -> Prop) `{ forall x, Decision (P x) } l:
+  Forall P l ->
+  @list_filter _ P _ l = l.
+Proof.
+  induction 1; auto.
+  simpl. destruct (decide (P x)); rewrite /filter; try congruence.
+Qed.
